progs/verif_evenodd_spec.v
@@ -1,8 +1,6 @@
 Require Import VST.floyd.proofauto.
 Require Import VST.progs.even.
 
-Require Import VST.floyd.Funspec_old_Notation.
-
 Instance CompSpecs : compspecs.
 Proof. make_compspecs prog. Defined.
 Definition Vprog : varspecs. mk_varspecs prog. Defined.
@@ -12,22 +10,22 @@ Local Open Scope assert.
 Definition odd_spec :=
  DECLARE _odd
   WITH z : Z, b: unit
-  PRE [ _n OF tuint]
-    PROP(0 <= z <= Int.max_signed) LOCAL(temp _n (Vint (Int.repr z))) SEP()
+  PRE [ tuint]
+    PROP(0 <= z <= Int.max_signed) PARAMS(Vint (Int.repr z)) SEP()
   POST [ tint ]
-    PROP() LOCAL(temp ret_temp (Vint (if Z.odd z then Int.one else Int.zero))) SEP().
+    PROP() RETURN(Vint (if Z.odd z then Int.one else Int.zero)) SEP().
 
 Definition even_spec :=
  DECLARE _even
   WITH z : Z
-  PRE [ _n OF tuint]
-    PROP(0 <= z <= Int.max_signed) LOCAL(temp _n (Vint (Int.repr z))) SEP()
+  PRE [ tuint]
+    PROP(0 <= z <= Int.max_signed) PARAMS(Vint (Int.repr z)) SEP()
   POST [ tint ]
-    PROP() LOCAL(temp ret_temp (Vint (if Z.even z then Int.one else Int.zero))) SEP().
+    PROP() RETURN (Vint (if Z.even z then Int.one else Int.zero)) SEP().
 
 Definition main_spec :=
  DECLARE _main
   WITH gv : globals
   PRE  [] main_pre prog tt gv
   POST [ tint ]
-    PROP() LOCAL(temp ret_temp (Vint (if Z.even 42 then Int.one else Int.zero))) SEP(has_ext tt).
+    PROP() RETURN (Vint (if Z.even 42 then Int.one else Int.zero)) SEP(has_ext tt).
