progs64/verif_field_loadstore.v
@@ -2,7 +2,6 @@
 Require Import VST.floyd.proofauto.
 Require Import VST.progs64.field_loadstore.
 
-Require Export VST.floyd.Funspec_old_Notation.
 Instance CompSpecs : compspecs. make_compspecs prog. Defined.
 Definition Vprog : varspecs. mk_varspecs prog. Defined.
 
@@ -15,10 +14,10 @@ Definition sub_spec (sub_id: ident) :=
   WITH v : val * list (val*val) , gv: globals
   PRE  []
         PROP  (is_int I8 Signed (snd (nth 1%nat (snd v) (Vundef, Vundef))))
-        LOCAL (gvars gv)
+        PARAMS() GLOBALS (gv)
         SEP   (data_at Ews t_struct_b v (gv _p))
   POST [ tvoid ]
-        PROP() LOCAL()
+        PROP() RETURN()
         SEP(data_at Ews t_struct_b (snd (nth 1%nat (snd v) (Vundef, Vundef)), snd v) (gv _p)).
 
 Definition sub_spec' (sub_id: ident) :=
@@ -26,10 +25,10 @@ Definition sub_spec' (sub_id: ident) :=
   WITH v : reptype t_struct_b, gv: globals
   PRE  []
         PROP  (is_int I8 Signed (proj_reptype _ (DOT _y2 SUB 1 DOT _x2) v))
-        LOCAL (gvars gv)
+        PARAMS() GLOBALS (gv)
         SEP   (data_at Ews t_struct_b v (gv _p))
   POST [ tvoid ]
-        PROP() LOCAL()
+        PROP() RETURN()
         SEP(data_at Ews t_struct_b
            (upd_reptype t_struct_b (DOT _y1) v
              (proj_reptype t_struct_b (StructField _x2 :: ArraySubsc 1 :: StructField _y2 :: nil) v))
